src/proof/iam_model/example_init.v
@@ -1,0 +1,14 @@
+From New.proof Require Export prelude.
+From New.proof.iam_model Require Export common.
+Require Export New.generatedproof.iam_model.example.
+From New.proof Require Import proof_prelude.
+
+Section proof.
+Context `{hG: heapGS Σ} `{!ffi_semantics _ _}.
+Context {sem : go.Semantics} {package_sem : example.Assumptions}.
+Collection W := sem + package_sem.
+
+#[global] Instance : IsPkgInit (iProp Σ) example := define_is_pkg_init True%I.
+#[global] Instance : GetIsPkgInitWf (iProp Σ) example := build_get_is_pkg_init_wf.
+
+End proof.
