src/proof/iam_model/snapshot.v
@@ -48,28 +48,113 @@ Proof.
     apply leibniz_equiv, size_empty_inv. lia.
 Qed.
 
-Lemma wp_State__Snapshot γ l resource dq attachments :
+Lemma own_iam_identity_frags_consistent γ auth_abs_identities abs_identities :
+  own_iam_identities_auth γ auth_abs_identities -∗
+  ([∗ map] identity ↦ policy_ids ∈ abs_identities,
+    own_iam_identity_frag γ identity 1 policy_ids) -∗
+  ⌜ ∀ identity policy_ids,
+    abs_identities !! identity = Some policy_ids →
+    auth_abs_identities !! identity = Some policy_ids ⌝ ∗
+  own_iam_identities_auth γ auth_abs_identities ∗
+  ([∗ map] identity ↦ policy_ids ∈ abs_identities,
+    own_iam_identity_frag γ identity 1 policy_ids).
+Proof.
+  revert auth_abs_identities.
+  induction abs_identities as [|identity policy_ids abs_identities Hfresh IH]
+    using map_ind; iIntros (auth_abs_identities) "Hauth Hfrags".
+  - rewrite big_sepM_empty. iSplit; [|iFrame].
+    iPureIntro. intros identity policy_ids Hlookup.
+    rewrite lookup_empty in Hlookup. done.
+  - rewrite big_sepM_insert //.
+    iDestruct "Hfrags" as "[Hfrag Hfrags]".
+    iDestruct (IH with "Hauth Hfrags")
+      as "(%Hrest & Hauth & Hfrags)".
+    iDestruct (own_identities_auth_frag_lookup with "Hauth Hfrag")
+      as %Hlookup_auth.
+    iSplit.
+    + iPureIntro. intros identity' policy_ids' Hlookup.
+      destruct (decide (identity' = identity)) as [->|Hne].
+      * rewrite lookup_insert_eq in Hlookup. inversion Hlookup. subst. done.
+      * assert (identity ≠ identity') as Hne' by congruence.
+        replace ((<[identity:=policy_ids]> abs_identities) !! identity')
+          with (abs_identities !! identity') in Hlookup.
+        2:{ symmetry. apply lookup_insert_ne. exact Hne'. }
+        apply Hrest. done.
+    + iFrame.
+Qed.
+
+Lemma own_iam_policy_frags_consistent γ auth_policies policies q_policy :
+  own_iam_policies_auth γ auth_policies -∗
+  ([∗ map] policy_id ↦ policy ∈ policies,
+    own_iam_policy_frag γ policy_id q_policy policy) -∗
+  ⌜ ∀ policy_id policy,
+    policies !! policy_id = Some policy →
+    auth_policies !! policy_id = Some policy ⌝ ∗
+  own_iam_policies_auth γ auth_policies ∗
+  ([∗ map] policy_id ↦ policy ∈ policies,
+    own_iam_policy_frag γ policy_id q_policy policy).
+Proof.
+  revert auth_policies.
+  induction policies as [|policy_id policy policies Hfresh IH]
+    using map_ind; iIntros (auth_policies) "Hauth Hfrags".
+  - rewrite big_sepM_empty. iSplit; [|iFrame].
+    iPureIntro. intros policy_id policy Hlookup.
+    rewrite lookup_empty in Hlookup. done.
+  - rewrite big_sepM_insert //.
+    iDestruct "Hfrags" as "[Hfrag Hfrags]".
+    iDestruct (IH with "Hauth Hfrags")
+      as "(%Hrest & Hauth & Hfrags)".
+    iDestruct (own_policies_auth_frag_lookup with "Hauth Hfrag")
+      as %Hlookup_auth.
+    iSplit.
+    + iPureIntro. intros policy_id' policy' Hlookup.
+      destruct (decide (policy_id' = policy_id)) as [->|Hne].
+      * rewrite lookup_insert_eq in Hlookup. inversion Hlookup. subst. done.
+      * assert (policy_id ≠ policy_id') as Hne' by congruence.
+        replace ((<[policy_id:=policy]> policies) !! policy_id')
+          with (policies !! policy_id') in Hlookup.
+        2:{ symmetry. apply lookup_insert_ne. exact Hne'. }
+        apply Hrest. done.
+    + iFrame.
+Qed.
+
+Lemma wp_State__Snapshot
+    γ l resource dq attachments abs_identities policies q_policy :
   {{{ "#Hiam" ∷ is_iam γ l ∗
-      "Hattachments" ∷ own_iam_attachments_frag γ resource dq attachments
+      "Hattachments" ∷ own_iam_attachments_frag γ resource dq attachments ∗
+      "Hidentity_map" ∷ ([∗ map] identity ↦ policy_ids ∈ abs_identities,
+        own_iam_identity_frag γ identity 1 policy_ids) ∗
+      "Hpolicy_map" ∷ ([∗ map] policy_id ↦ policy ∈ policies,
+        own_iam_policy_frag γ policy_id q_policy policy)
   }}}
     l @! (go.PointerType iammodel.State) @! "Snapshot" #()
-  {{{ identities_l policies_l phys_identities abs_identities policies,
+  {{{ identities_l policies_l phys_identities snap_abs_identities snap_policies,
       RET (#identities_l, #policies_l);
       "Hattachments" ∷ own_iam_attachments_frag γ resource dq attachments ∗
-      "Hidentities" ∷ identities_l ↦$ phys_identities ∗
-      "Hidentities_inner" ∷ ([∗ map] policy_ids_l; policy_ids ∈
-        phys_identities; abs_identities, policy_ids_l ↦$ policy_ids) ∗
-      "Hpolicies" ∷ policies_l ↦$ policies ∗
+      "Hidentity_map" ∷ ([∗ map] identity ↦ policy_ids ∈ abs_identities,
+        own_iam_identity_frag γ identity 1 policy_ids) ∗
+      "Hpolicy_map" ∷ ([∗ map] policy_id ↦ policy ∈ policies,
+        own_iam_policy_frag γ policy_id q_policy policy) ∗
+      "Hidentities_l" ∷ identities_l ↦$ phys_identities ∗
+      "Hidentities_l_inner" ∷ ([∗ map] policy_ids_l; policy_ids ∈
+        phys_identities; snap_abs_identities, policy_ids_l ↦$ policy_ids) ∗
+      "Hpolicies_l" ∷ policies_l ↦$ snap_policies ∗
+      "%Hidentity_map_consistent" ∷ ⌜ ∀ identity policy_ids,
+        abs_identities !! identity = Some policy_ids →
+        snap_abs_identities !! identity = Some policy_ids ⌝ ∗
+      "%Hpolicy_map_consistent" ∷ ⌜ ∀ policy_id policy,
+        policies !! policy_id = Some policy →
+        snap_policies !! policy_id = Some policy ⌝ ∗
       "%Hattachments_consistent" ∷ ⌜
-        attachments = attachment_counts abs_identities policies resource ⌝ ∗
+        attachments = attachment_counts snap_abs_identities snap_policies resource ⌝ ∗
       "%Hidentities_with_access" ∷ ⌜
         dom attachments =
         dom (filter (λ '(_, policy_ids),
-          attached_policies_for_resource policies policy_ids resource ≠ ∅)
-          abs_identities) ⌝
+          attached_policies_for_resource snap_policies policy_ids resource ≠ ∅)
+          snap_abs_identities) ⌝
   }}}.
 Proof.
-  iIntros (Φ) "(#Hiam & Hattachments) HΦ".
+  iIntros (Φ) "(#Hiam & Hattachments & Hidentity_map & Hpolicy_map) HΦ".
   iDestruct "Hiam" as (mu_l) "[#Hmu #Hiam_inv]".
   wp_method_call. rewrite /iammodel.State__Snapshotⁱᵐᵖˡ. wp_call.
   wp_apply wp_with_defer as "%defer Hdefer". simpl subst. wp_auto.
@@ -80,6 +165,14 @@ Proof.
   iDestruct (own_attachments_frag_valid_pure with
     "Hinv_Hown_attachments_auth Hattachments") as
     %[Hattachments_consistent _].
+  iDestruct (own_iam_identity_frags_consistent with
+    "Hinv_Hown_identities_auth Hidentity_map")
+    as "(%Hidentity_map_consistent & Hinv_Hown_identities_auth &
+      Hidentity_map)".
+  iDestruct (own_iam_policy_frags_consistent with
+    "Hinv_Hown_policies_auth Hpolicy_map")
+    as "(%Hpolicy_map_consistent & Hinv_Hown_policies_auth &
+      Hpolicy_map)".
   rewrite exception_do_unseal /exception_do_def.
   rewrite do_return_unseal.
   wp_pures.
@@ -100,7 +193,9 @@ Proof.
     iEval (rewrite is_pkg_init_unfold /=).
     iSplit; [iModIntro; iEval (rewrite !is_pkg_init_unfold /=); done|done]. }
   iApply "HΦ". iFrame.
-  iPureIntro. split.
+  iPureIntro. repeat split.
+  - exact Hidentity_map_consistent.
+  - exact Hpolicy_map_consistent.
   - done.
   - rewrite Hattachments_consistent.
     apply attachment_counts_dom_nonempty.
